pulse/lib/pulse/lib/Pulse.Lib.Pervasives.fst
@@ -25,6 +25,8 @@ include PulseCore.FractionalPermission
 include PulseCore.Observability
 include FStar.Ghost
 
+module GSet = FStar.GhostSet
+
 (* Pulse will currently not recognize calls to anything other than
 top-level names, so this allows to force it. *)
 val perform
@@ -41,22 +43,22 @@ let perform_ghost f = f ()
 
 (* TEMPORARY! REMOVE! *)
 let inames_ext (is1 is2 : inames)
-  : Lemma (requires forall i. Set.mem i is1 <==> Set.mem i is2)
+  : Lemma (requires forall i. GSet.mem i is1 <==> GSet.mem i is2)
           (ensures is1 == is2)
           [SMTPat (is1 == is2)]
-  = Set.lemma_equal_intro is1 is2
+  = GSet.lemma_equal_intro is1 is2
 
 let inames_join_emp_r (is1 : inames)
   : Lemma (join_inames is1 emp_inames == is1) [SMTPat (join_inames is1 emp_inames)]
-  = Set.lemma_equal_intro (join_inames is1 emp_inames) is1
+  = GSet.lemma_equal_intro (join_inames is1 emp_inames) is1
 
 let inames_join_emp_l (is1 : inames)
   : Lemma (join_inames emp_inames is1 == is1) [SMTPat (join_inames emp_inames is1)]
-  = Set.lemma_equal_intro (join_inames emp_inames is1) is1
+  = GSet.lemma_equal_intro (join_inames emp_inames is1) is1
 
 let inames_join_self (is1 : inames)
   : Lemma (join_inames is1 is1 == is1) [SMTPat (join_inames is1 is1)]
-  = Set.lemma_equal_intro (join_inames is1 is1) is1
+  = GSet.lemma_equal_intro (join_inames is1 is1) is1
 
 //
 // Native extraction in the Rust backend
